Views for unions

examples/steel/arraystructs/Steel.C.Union.fst
@@ -480,87 +480,81 @@ let unaddr_of_union_field
 
 let union_view_to_view_prop
   (#a:Type) (#b: a -> Type) (#p:(k:a -> pcm (b k)))
-  (#view_t:a -> Type) (field_view:(k:a -> sel_view (p k) (view_t k)))
+  (#view_t:a -> Type) (case_view:(k:a -> sel_view (p k) (view_t k) false))
 : union p -> Tot prop
-= fun u -> forall k. case_refinement_f p k u ==> (field_view k).to_view_prop (u k)
+= fun u ->
+  u =!= one (union_pcm p) /\
+  (forall k. case_refinement_f p k u ==> (case_view k).to_view_prop (u k))
 
 let union_view_to_view
   (#a:Type) (#b: a -> Type) (#p:(k:a -> pcm (b k)))
-  (#view_t:a -> Type) (field_view:(k:a -> sel_view (p k) (view_t k)))
+  (#view_t:a -> Type) (case_view:(k:a -> sel_view (p k) (view_t k) false))
   (case_of:(u:union p -> k:a{case_refinement_f p k u}))
-: refine (union p) (union_view_to_view_prop field_view) -> dtuple2 a view_t
+: refine (union p) (union_view_to_view_prop case_view) -> dtuple2 a view_t
 = fun u ->
   let k = case_of u in
-  (|k, (field_view k).to_view (u k)|)
+  (|k, (case_view k).to_view (u k)|)
 
 let union_view_to_carrier
   (#a:eqtype) (#b: a -> Type) (#p:(k:a -> pcm (b k)))
-  (#view_t:a -> Type) (field_view:(k:a -> s:sel_view (p k) (view_t k)
-  //{
-  //  ~ (s.to_view_prop (one (p k)))
-  //  // TODO Can we add this to the definition of a view?
-  //}))
-  ))
-: dtuple2 a view_t -> refine (union p) (union_view_to_view_prop field_view)
+  (#view_t:a -> Type) (case_view:(k:a -> sel_view (p k) (view_t k) false))
+: dtuple2 a view_t -> refine (union p) (union_view_to_view_prop case_view)
 = fun (|k, x|) ->
-  let u: union p = field_to_union_f p k ((field_view k).to_carrier x) in
+  let u: union p = field_to_union_f p k ((case_view k).to_carrier x) in
   assert (case_refinement_f p k u);
-  assert (u k == (field_view k).to_carrier x);
-  assert ((field_view k).to_view_prop ((field_view k).to_carrier x));
-  assert ((field_view k).to_view_prop (u k));
+  assert (u k == (case_view k).to_carrier x);
+  assert ((case_view k).to_view_prop ((case_view k).to_carrier x));
+  assert ((case_view k).to_view_prop (u k));
   // If (to_carrier x =!= one (p k)), then k is the unique k s.t. case_refinement p k u
   // and we are done.
   // If (to_carrier x == one (p k)), then must show that
   //   forall k. to_view_prop (u k)
   u
 
-// let union_view_to_carrier_not_one
-//   (#a:eqtype) (#b: a -> Type) (#p:(k:a -> pcm (b k)))
-//   (#view_t:a -> Type) (field_view:(k:a -> s:sel_view (p k) (view_t k)
-//   //{
-//   //  ~ (s.to_view_prop (one (p k)))
-//   //  // TODO Can we add this to the definition of a view?
-//   //}))
-//   ))
-// : u:dtuple2 a view_t -> Lemma (union_view_to_carrier field_view u =!= one (union_pcm p))
-// = fun _ -> ()
-
-let union_view_to_view_frame
+let union_view_to_carrier_not_one
   (#a:eqtype) (#b: a -> Type) (#p:(k:a -> pcm (b k)))
-  (#view_t:a -> Type) (field_view:(k:a -> s:sel_view (p k) (view_t k)
+  (#view_t:a -> Type) (case_view:(k:a -> sel_view (p k) (view_t k) false))
   //{
   //  ~ (s.to_view_prop (one (p k)))
   //  // TODO Can we add this to the definition of a view?
   //}))
-  ))
+: u:dtuple2 a view_t -> Lemma (union_view_to_carrier case_view u =!= one (union_pcm p))
+= fun _ -> ()
+
+let union_view_to_view_frame
+  (#a:eqtype) (#b: a -> Type) (#p:(k:a -> pcm (b k)))
+  (#view_t:a -> Type) (case_view:(k:a -> sel_view (p k) (view_t k) false))
+  //{
+  //  ~ (s.to_view_prop (one (p k)))
+  //  // TODO Can we add this to the definition of a view?
+  //}))
   (case_of:(u:union p -> k:a{case_refinement_f p k u}))
 : (v: dtuple2 a view_t) ->
   (u: union p) ->
   Lemma
-    (requires composable (union_pcm p) (union_view_to_carrier field_view v) u)
+    (requires composable (union_pcm p) (union_view_to_carrier case_view v) u)
     (ensures 
-      union_view_to_view_prop field_view (op (union_pcm p) (union_view_to_carrier field_view v) u) /\
-      union_view_to_view field_view case_of
-        (op (union_pcm p) (union_view_to_carrier field_view v) u) == v)
+      union_view_to_view_prop case_view (op (union_pcm p) (union_view_to_carrier case_view v) u) /\
+      union_view_to_view case_view case_of
+        (op (union_pcm p) (union_view_to_carrier case_view v) u) == v)
 = fun (|k, x|) u ->
-  assert (composable (p k) ((field_view k).to_carrier x) (u k));
-  (field_view k).to_view_frame x (u k);
+  assert (composable (p k) ((case_view k).to_carrier x) (u k));
+  (case_view k).to_view_frame x (u k);
   ()
 
 let union_view
   (#a:eqtype) (#b: a -> Type) (#p:(k:a -> pcm (b k)))
-  (#view_t:a -> Type) (field_view:(k:a -> s:sel_view (p k) (view_t k)
+  (#view_t:a -> Type) (case_view:(k:a -> sel_view (p k) (view_t k) false))
   //{
   //  ~ (s.to_view_prop (one (p k)))
   //  // TODO Can we add this to the definition of a view?
   //}))
-  ))
   (case_of:(u:union p -> k:a{case_refinement_f p k u}))
-: Tot (sel_view (union_pcm p) (dtuple2 a view_t))
+: Tot (sel_view (union_pcm p) (dtuple2 a view_t) false)
 = {
-  to_view_prop = union_view_to_view_prop field_view;
-  to_view = union_view_to_view field_view case_of;
-  to_carrier = union_view_to_carrier field_view;
-  to_carrier_not_one = (fun _ -> ()); // union_view_to_carrier_not_one field_view;
-  to_view_frame = union_view_to_view_frame field_view case_of;
+  to_view_prop = union_view_to_view_prop case_view;
+  to_view = union_view_to_view case_view case_of;
+  to_carrier = union_view_to_carrier case_view;
+  to_carrier_not_one = ();
+  to_view_frame = union_view_to_view_frame case_view case_of;
 }
